tests/fstar/misc/Constants.fst
@@ -18,30 +18,30 @@ let x2_body : result u32 = Return 3
 let x2_c : u32 = eval_global x2_body
 
 (** [constants::incr]: forward function *)
-let incr_fwd (n : u32) : result u32 =
+let incr (n : u32) : result u32 =
   u32_add n 1
 
 (** [constants::X3] *)
-let x3_body : result u32 = incr_fwd 32
+let x3_body : result u32 = incr 32
 let x3_c : u32 = eval_global x3_body
 
 (** [constants::mk_pair0]: forward function *)
-let mk_pair0_fwd (x : u32) (y : u32) : result (u32 & u32) =
+let mk_pair0 (x : u32) (y : u32) : result (u32 & u32) =
   Return (x, y)
 
 (** [constants::Pair] *)
-type pair_t (t1 t2 : Type0) = { pair_x : t1; pair_y : t2; }
+type pair_t (t1 t2 : Type0) = { x : t1; y : t2; }
 
 (** [constants::mk_pair1]: forward function *)
-let mk_pair1_fwd (x : u32) (y : u32) : result (pair_t u32 u32) =
-  Return { pair_x = x; pair_y = y }
+let mk_pair1 (x : u32) (y : u32) : result (pair_t u32 u32) =
+  Return { x = x; y = y }
 
 (** [constants::P0] *)
-let p0_body : result (u32 & u32) = mk_pair0_fwd 0 1
+let p0_body : result (u32 & u32) = mk_pair0 0 1
 let p0_c : (u32 & u32) = eval_global p0_body
 
 (** [constants::P1] *)
-let p1_body : result (pair_t u32 u32) = mk_pair1_fwd 0 1
+let p1_body : result (pair_t u32 u32) = mk_pair1 0 1
 let p1_c : pair_t u32 u32 = eval_global p1_body
 
 (** [constants::P2] *)
@@ -49,26 +49,26 @@ let p2_body : result (u32 & u32) = Return (0, 1)
 let p2_c : (u32 & u32) = eval_global p2_body
 
 (** [constants::P3] *)
-let p3_body : result (pair_t u32 u32) = Return { pair_x = 0; pair_y = 1 }
+let p3_body : result (pair_t u32 u32) = Return { x = 0; y = 1 }
 let p3_c : pair_t u32 u32 = eval_global p3_body
 
 (** [constants::Wrap] *)
-type wrap_t (t : Type0) = { wrap_val : t; }
+type wrap_t (t : Type0) = { value : t; }
 
 (** [constants::Wrap::{0}::new]: forward function *)
-let wrap_new_fwd (t : Type0) (val0 : t) : result (wrap_t t) =
-  Return { wrap_val = val0 }
+let wrap_new (t : Type0) (value : t) : result (wrap_t t) =
+  Return { value = value }
 
 (** [constants::Y] *)
-let y_body : result (wrap_t i32) = wrap_new_fwd i32 2
+let y_body : result (wrap_t i32) = wrap_new i32 2
 let y_c : wrap_t i32 = eval_global y_body
 
 (** [constants::unwrap_y]: forward function *)
-let unwrap_y_fwd : result i32 =
-  Return y_c.wrap_val
+let unwrap_y : result i32 =
+  Return y_c.value
 
 (** [constants::YVAL] *)
-let yval_body : result i32 = unwrap_y_fwd
+let yval_body : result i32 = unwrap_y
 let yval_c : i32 = eval_global yval_body
 
 (** [constants::get_z1::Z1] *)
@@ -76,11 +76,11 @@ let get_z1_z1_body : result i32 = Return 3
 let get_z1_z1_c : i32 = eval_global get_z1_z1_body
 
 (** [constants::get_z1]: forward function *)
-let get_z1_fwd : result i32 =
+let get_z1 : result i32 =
   Return get_z1_z1_c
 
 (** [constants::add]: forward function *)
-let add_fwd (a : i32) (b : i32) : result i32 =
+let add (a : i32) (b : i32) : result i32 =
   i32_add a b
 
 (** [constants::Q1] *)
@@ -92,19 +92,19 @@ let q2_body : result i32 = Return q1_c
 let q2_c : i32 = eval_global q2_body
 
 (** [constants::Q3] *)
-let q3_body : result i32 = add_fwd q2_c 3
+let q3_body : result i32 = add q2_c 3
 let q3_c : i32 = eval_global q3_body
 
 (** [constants::get_z2]: forward function *)
-let get_z2_fwd : result i32 =
-  let* i = get_z1_fwd in let* i0 = add_fwd i q3_c in add_fwd q1_c i0
+let get_z2 : result i32 =
+  let* i = get_z1 in let* i0 = add i q3_c in add q1_c i0
 
 (** [constants::S1] *)
 let s1_body : result u32 = Return 6
 let s1_c : u32 = eval_global s1_body
 
 (** [constants::S2] *)
-let s2_body : result u32 = incr_fwd s1_c
+let s2_body : result u32 = incr s1_c
 let s2_c : u32 = eval_global s2_body
 
 (** [constants::S3] *)
@@ -112,6 +112,6 @@ let s3_body : result (pair_t u32 u32) = Return p3_c
 let s3_c : pair_t u32 u32 = eval_global s3_body
 
 (** [constants::S4] *)
-let s4_body : result (pair_t u32 u32) = mk_pair1_fwd 7 8
+let s4_body : result (pair_t u32 u32) = mk_pair1 7 8
 let s4_c : pair_t u32 u32 = eval_global s4_body
 
